Dafny/examples/Challenge9/Challenge9PropertiesVulnExample.i.dfy
@@ -1,0 +1,67 @@
+include "Challenge9CodeExample.i.dfy"
+include "../../LLVM/llvmNEW.i.dfy"
+include "../../LLVM/types.s.dfy"
+include "../../Libraries/Seqs.s.dfy"
+
+module challenge9PropertiesExample{
+    import opened challenge9CodeExample
+    import opened LLVM_def_NEW
+    import opened types
+    import opened Collections__Seqs_s
+
+
+lemma isPatchIsSuccesful()
+    ensures forall s,b :: && ValidState(s) 
+                          && validConfig(s) 
+                          && b == [s] + evalCodeFn(entrySimplVuln(),s) ==> !miniSpec(s,b)
+{
+    forall s:State,b | && ValidState(s) && validConfig(s) && b == [s] + evalCodeFn(entrySimplVuln(),s)
+        ensures !miniSpec(s,b);
+     {
+        var b := unwrapPatch(s);
+        assert !miniSpec(s,b);
+     }
+}
+
+
+    lemma unwrapPatch(s:State) returns (b:Behavior)
+        requires ValidState(s);
+        requires validConfig(s);
+        ensures b == [s] + evalCodeFn(entrySimplVuln(),s);
+        ensures !miniSpec(s,b);
+    {
+        var config := allVariablesConfig();
+        b := [s] + evalCodeFn(entrySimplVuln(),s);
+        // assert |b| == 7;
+        assert NextStep(b[0],b[1],evalInsStep((LOAD(config.ops["var_0"],1,config.ops["var_num_connections"]))));
+        assert NextStep(b[1],b[2],evalInsStep((ZEXT(config.ops["var_conv"],1,config.ops["var_0"],4))));
+       
+        assert NextStep(b[2],b[3],evalInsStep((STORE(D(Int(1,IntType(1,false))),config.ops["var_retval"]))));
+
+        
+        assert NextStep(b[3],b[4],evalInsStep((LOAD(config.ops["var_28"],1,config.ops["var_retval"]))));
+        assert NextStep(b[4],b[5],evalInsStep((RET(config.ops["var_28"]))));
+            
+            // assert (OperandContents(last(b),config.ops["var_0"]).val >= 255 && OperandContents(last(b),config.ops["var_0"]).val < 0x8000_0000) ==> OperandContents(last(b),config.ops["var_28"]).val == 0;
+            // assert OperandContents(last(b),config.ops["var_0"]).val < 255 ==> OperandContents(last(b),config.ops["var_28"]).val == 1;
+    }
+
+    predicate miniSpec(s:State,b:Behavior)
+    {
+        reveal_ValidBehavior();
+        var config := allVariablesConfig();
+       && ValidState(s)
+       && validConfig(s)
+       && ValidBehavior(b)
+       && |b| > 0
+       && ValidOperand(last(b),allVariablesConfig().ops["var_28"])
+       && OperandContents(last(b),allVariablesConfig().ops["var_28"]).Int?
+       && ValidOperand(last(b),allVariablesConfig().ops["var_0"])
+       && OperandContents(last(b),allVariablesConfig().ops["var_0"]).Int?
+       //
+       && OperandContents(last(b),allVariablesConfig().ops["var_28"]).val == 1
+       && (OperandContents(last(b),config.ops["var_0"]).val >= 255 && OperandContents(last(b),config.ops["var_0"]).val < 0x8000_0000)
+    }
+
+
+}
